src/type_directed_translation.v
@@ -1,0 +1,6 @@
+Require Import DTDT.syntax.
+Require Import DTDT.big_step_eval.
+Require Import DTDT.semantic_rules.
+
+(* --- Type directed translation from surface language to internal language -------------- *)
+
